DS: finished implementation and proof of third protocol step
To make it work, it was necessary to adapt the label of the communication key
generated by the initiator (because we can't definitely tell the sk label of what
we assume to be the responders public key - malicious server may send us crap).
Furthermore, I have a headache from trying to proof the correctness of the
third step...

denning-sacco/DS.Protocol.fst
@@ -88,6 +88,76 @@ let server_send_msg_2 srv msg1_idx =
       (msg2_idx, new_sess_idx, c_out)
   )
   | _ -> error "[srv_send_m2] wrong message"
+#pop-options
+
+#push-options "--z3rlimit 200"
+let trigger_event_send_key (prev:timestamp) (a b srv:principal) (pk_a pk_b ck:bytes) (t:timestamp) (clock_cnt:nat) (cert_a cert_b:msg ds_global_usage prev public) (verk_srv:verify_key ds_global_usage prev (readers [P srv]) "DS.sig_key") :
+  LCrypto timestamp (pki ds_preds)
+  (requires (fun t0 -> prev < trace_len t0 /\
+    (clock_cnt <= recv_msg_2_delay) /\
+    parse_sigval_ cert_a == Success (CertA a pk_a t) /\
+    parse_sigval_ cert_b == Success (CertB b pk_b t) /\
+    (can_flow prev (readers [P srv]) public \/
+      sign_pred ds_usage_preds prev "DS.sig_key" verk_srv cert_a /\
+      sign_pred ds_usage_preds prev "DS.sig_key" verk_srv cert_b) /\
+      was_rand_generated_before (trace_len t0) ck (join (readers [P a]) (get_sk_label ds_key_usages pk_b)) (aead_usage "DS.comm_key")
+  ))
+  (ensures (fun t0 now t1 -> now == trace_len t0 /\ trace_len t1 == trace_len t0 + 1 /\
+    did_event_occur_at now a (event_send_key a b srv pk_a pk_b ck t clock_cnt))) =
+  let now = global_timestamp () in
+  let event = event_send_key a b srv pk_a pk_b ck t clock_cnt in
+  publishable_readers_implies_corruption #prev [P srv];
+  assert(corrupt_id prev (P srv) \/ sign_pred ds_usage_preds prev "DS.sig_key" verk_srv cert_a);
+  assert(corrupt_id prev (P srv) \/ sign_pred ds_usage_preds prev "DS.sig_key" verk_srv cert_b);
+  readers_is_injective srv;
+  verification_key_label_lemma ds_global_usage prev verk_srv (readers [P srv]);
+  assert(get_signkey_label ds_key_usages verk_srv == readers [P srv]);
+  assert(corrupt_id prev (P srv)
+    \/ did_event_occur_at t srv (event_certify a b srv pk_a pk_b t 0));
+  trigger_event #ds_preds a event;
+  now
+
+let initiator_send_msg_3_helper (now:timestamp) (a b srv:principal) (ck pk_a pk_b:bytes) (t:timestamp) (cert_a sig_cert_a cert_b sig_cert_b:msg ds_global_usage now public) (sigk_a:sign_key ds_global_usage now (readers [P a]) "DS.sig_key") (n_sig n_pke:bytes) (clock_cnt:nat) (c_rm2:clock) :
+  LCrypto (si:timestamp & c_out:clock) (pki ds_preds)
+  (requires (fun t0 -> now == trace_len t0 /\
+    clock_cnt == (clock_get c_rm2) /\ clock_cnt <= recv_msg_2_delay /\
+    was_rand_generated_before now ck (join (readers [P a]) (get_sk_label ds_key_usages pk_b)) (aead_usage "DS.comm_key") /\
+    is_msg ds_global_usage now pk_b public /\
+    did_event_occur_before now a (event_send_key a b srv pk_a pk_b ck t clock_cnt) /\
+    is_labeled ds_global_usage now n_sig (readers [P a]) /\
+    is_pke_nonce ds_global_usage now n_pke (readers [P a])
+  ))
+  (ensures (fun t0 (|si,c_out|) t1 ->
+     si == trace_len t0 /\
+     trace_len t1 = trace_len t0 + 1 /\
+     clock_get c_out = clock_cnt + 1)) =
+  let l_ck = join (readers [P a]) (get_sk_label ds_key_usages pk_b) in
+
+  // create and sign sigval containing communication key
+  let sv_comm_key = CommKey ck t in
+  assert(was_rand_generated_before now ck l_ck (aead_usage "DS.comm_key"));
+  rand_is_secret #ds_global_usage #now #l_ck #(aead_usage "DS.comm_key") ck;
+  assert(is_msg ds_global_usage now ck l_ck);
+  let ser_comm_key = serialize_sigval now sv_comm_key l_ck in
+  readers_is_injective a;
+  assert(get_signkey_label ds_key_usages (vk #ds_global_usage #now #(readers [P a]) sigk_a) == readers [P a]);
+  assert(was_rand_generated_before now ck l_ck (aead_usage "DS.comm_key"));
+  assert(did_event_occur_before now a (event_send_key a b srv pk_a pk_b ck t (clock_get c_rm2)));
+  parse_serialize_sigval_lemma now sv_comm_key l_ck;
+  assert(can_sign now "DS.sig_key" (vk #ds_global_usage #now #(readers [P a]) sigk_a) ser_comm_key);
+  let sig_comm_key = sign #ds_global_usage #now #(readers [P a]) #l_ck sigk_a n_sig ser_comm_key in
+
+  // create and encrypt encval containing signed sigval with communication key
+  let ev_comm_key = encval_comm_key ser_comm_key sig_comm_key in
+  assert(is_msg ds_global_usage now ck (get_sk_label ds_key_usages pk_b));
+  assert(can_flow now (get_label ds_key_usages ev_comm_key) (readers [P a]));
+  let c_comm_key = pke_enc #ds_global_usage #now #(readers [P a]) pk_b n_pke ev_comm_key in
+
+  // create and send third message
+  let msg3 = Msg3 cert_a sig_cert_a cert_b sig_cert_b c_comm_key in
+  let ser_msg3 = serialize_msg now msg3 in
+
+  SR.send #now c_rm2 a b ser_msg3
 
 let initiator_send_msg_3 c_in a msg2_idx a_si =
   // get and parse initiator session
@@ -122,18 +192,14 @@ let initiator_send_msg_3 c_in a msg2_idx a_si =
                   else
                     // generate communication key
                     let prev = now in
-                    let (|_,ck|) = rand_gen #ds_preds (readers [P a; P b]) (aead_usage "DS.comm_key") in
+                    let l_ck = join (readers [P a]) (get_sk_label ds_key_usages pk_b) in
+                    let (|_,ck|) = rand_gen #ds_preds l_ck (aead_usage "DS.comm_key") in
 
                     // trigger event 'send_key'
-                    let event = event_send_key a b srv pk_a pk_b ck t (clock_get c_rm2) in
-                    let now = global_timestamp () in
-                    readers_is_injective srv;
-                    assert(can_flow prev (readers [P srv]) public \/ sign_pred ds_usage_preds prev "DS.sig_key" verk_srv cert_a);
-                    assert(can_flow prev (readers [P srv]) public \/ sign_pred ds_usage_preds prev "DS.sig_key" verk_srv cert_b);
-                    publishable_readers_implies_corruption #prev [P srv];
-                    assert(corrupt_id prev (P srv) \/ sign_pred ds_usage_preds prev "DS.sig_key" verk_srv cert_a);
-                    assert(corrupt_id prev (P srv) \/ sign_pred ds_usage_preds prev "DS.sig_key" verk_srv cert_b);
-                    trigger_event #ds_preds a event;
+                    parse_sigval_lemma cert_a;
+                    parse_sigval_lemma cert_b;
+                    let clock_cnt_event = clock_get c_rm2 in
+                    let t_event = trigger_event_send_key prev a b srv pk_a pk_b ck t clock_cnt_event cert_a cert_b verk_srv in
 
                     // look up sign key of initiator and generate sign nonce
                     let now = global_timestamp () in
@@ -143,25 +209,19 @@ let initiator_send_msg_3 c_in a msg2_idx a_si =
                     // generate pke nonce
                     let (|_,n_pke|) = rand_gen #ds_preds (readers [P a]) (nonce_usage "PKE_NONCE") in
 
-                    // create and sign sigval containing communication key
-                    let sv_comm_key = CommKey ck t in
-                    let now = global_timestamp () in
-                    let ser_comm_key = serialize_sigval now sv_comm_key (readers [P a; P b]) in
-                    let sig_comm_key = sign #ds_global_usage #now #(readers [P a]) #(readers [P a; P b]) sigk_a n_sig ser_comm_key in
-
-                    // create and encrypt encval containing signed sigval with communication key
-                    let ev_comm_key = encval_comm_key ser_comm_key sig_comm_key in
-                    let c_comm_key = pke_enc #ds_global_usage #now #(readers [P a]) pk_b n_pke ev_comm_key in
-
                     // create and send third message
-                    let msg3 = Msg3 cert_a sig_cert_a cert_b sig_cert_b c_comm_key in
-                    let ser_msg3 = serialize_msg now msg3 in
-
-                    let (|msg3_idx,c_out|) = SR.send #now c_rm2 a b ser_msg3 in
+                    let now = global_timestamp () in
+                    let cert_a:msg ds_global_usage now public = cert_a in
+                    let sig_cert_a:msg ds_global_usage now public = sig_cert_a in
+                    let cert_b:msg ds_global_usage now public = cert_b in
+                    let sig_cert_b:msg ds_global_usage now public = sig_cert_b in
+                    let (|msg3_idx,c_out|) = initiator_send_msg_3_helper now a b srv ck pk_a pk_b t cert_a sig_cert_a cert_b sig_cert_b sigk_a n_sig n_pke clock_cnt_event c_rm2 in
 
                     // update initiator session
-                    let st_i_sent_m3 = InitiatorSentMsg3 b ck in
+                    let st_i_sent_m3 = InitiatorSentMsg3 b srv ck in
                     let now = global_timestamp () in
+                    assert(corrupt_id prev (P srv) \/ is_pub_enc_key t pk_b b);
+                    sk_label_lemma ds_global_usage t pk_b (readers [P b]);
                     let ser_st = serialize_session_st now a a_si a_vi st_i_sent_m3 in
 
                     update_session #ds_preds #now a a_si a_vi ser_st;
