denning-sacco/DS.Sessions.fst
@@ -2,26 +2,31 @@ module DS.Sessions
 
 
 let serialize_session_st i p si vi st =
+  let l = readers [V p si vi] in
   match st with
   | InitiatorSentMsg1 b srv ->
     let tag = str_to_bytes #i "i_sent_m1" in
     let b_bytes = str_to_bytes #i b in
     let srv_bytes = str_to_bytes #i srv in
-    concat #i #(readers [V p si vi]) tag (concat #i #(readers [V p si vi]) b_bytes srv_bytes)
+    concat #i #l tag (concat #i #l b_bytes srv_bytes)
   | AuthServerSentMsg2 a b ->
     let tag = str_to_bytes #i "srv_sent_m2" in
     let a_bytes = str_to_bytes #i a in
     let b_bytes = str_to_bytes #i b in
-    concat #i #(readers [V p si vi]) tag (concat #i #(readers [V p si vi]) a_bytes b_bytes)
-  | InitiatorSentMsg3 b ck ->
+    concat #i #l tag (concat #i #l a_bytes b_bytes)
+  | InitiatorSentMsg3 b srv ck ->
     let tag = str_to_bytes #i "i_sent_m3" in
     let b_bytes = str_to_bytes #i b in
-    concat #i #(readers [V p si vi]) tag (concat #i #(readers [V p si vi]) b_bytes ck)
+    let srv_bytes = str_to_bytes #i srv in
+    LC.can_flow_transitive i (LC.get_label M.ds_key_usages ck) (readers [P p]) l;
+    LC.includes_can_flow_lemma i [P p] [V p si vi];
+    assert(covers (P p) (V p si vi)); // OK??
+    concat #i #l tag (concat #i #l b_bytes (concat #i #l srv_bytes ck))
   | ResponderRecvedMsg3 a ck ->
     let tag = str_to_bytes #i "r_rcvd_m3" in
     let a_bytes = str_to_bytes #i a in
-    LC.can_flow_transitive i (LC.get_label M.ds_key_usages ck) (readers [P p]) (readers [V p si vi]);
-    concat #i #(readers [V p si vi]) tag (concat #i #(readers [V p si vi]) a_bytes ck)
+    LC.can_flow_transitive i (LC.get_label M.ds_key_usages ck) (readers [P p]) l;
+    concat #i #l tag (concat #i #l a_bytes ck)
 
 let parse_session_st sst =
   split sst `bind` (fun (tag_bytes, rest) ->
@@ -38,9 +43,11 @@ let parse_session_st sst =
     bytes_to_string b_bytes `bind` (fun b ->
     Success (AuthServerSentMsg2 a b))))
   | "i_sent_m3" ->
-    split rest `bind` (fun (b_bytes, ck) ->
+    split rest `bind` (fun (b_bytes, rest) ->
+    split rest `bind`(fun (srv_bytes, ck) ->
     bytes_to_string b_bytes `bind` (fun b ->
-    Success (InitiatorSentMsg3 b ck)))
+    bytes_to_string srv_bytes `bind` (fun srv ->
+    Success (InitiatorSentMsg3 b srv ck)))))
   | "r_rcvd_m3" ->
     split rest `bind` (fun (a_bytes, ck) ->
     bytes_to_string a_bytes `bind` (fun a ->
@@ -49,7 +56,10 @@ let parse_session_st sst =
   ))
 
 let parse_serialize_session_st_lemma i p si vi st =
+  let l = (readers [V p si vi]) in
   match st with
+  | InitiatorSentMsg3 b srv ck ->
+    LC.can_flow_transitive i (LC.get_label M.ds_key_usages ck) (readers [P p]) l
   | ResponderRecvedMsg3 a ck ->
-    LC.can_flow_transitive i (LC.get_label M.ds_key_usages ck) (readers [P p]) (readers [V p si vi])
+    LC.can_flow_transitive i (LC.get_label M.ds_key_usages ck) (readers [P p]) l
   | _ -> ()
